Progress on Asm syntactic linking proof

games/AsmLinking.v
@@ -10,12 +10,295 @@ Require Import Asm.
 Require Import RTS.
 Require Import ModuleSemantics.
 Require Import Smallstep.
+Require Import OptionRel.
 
 Definition asm p : modsem (li_asm -o li_asm) :=
   Behavior.of (Asm.semantics p).
 
 Require Import Maps.
 Require Import List.
+Require Import BoolRel.
+
+Global Existing Instance Genv.Linker_genv.
+
+Record Senv_le ge1 ge2 : Prop :=
+  {
+    Senv_le_find_symbol i:
+      option_le eq (Senv.find_symbol ge1 i) (Senv.find_symbol ge2 i);
+    Senv_le_public_symbol i:
+      leb (Senv.public_symbol ge1 i) (Senv.public_symbol ge2 i);
+    Senv_le_block_is_volatile i:
+      option_le eq (Senv.block_is_volatile ge1 i) (Senv.block_is_volatile ge2 i);
+  }.
+
+Section GENV_REL.
+  Context {F V} `{LF: Linker F} `{LV: Linker V} `{FI: FundefIsInternal F}.
+
+  Global Instance find_symbol_linkorder:
+    Monotonic
+      (@Genv.find_symbol F V)
+      (linkorder ++> - ==> option_le eq).
+  Proof.
+    intros ge1 ge2 Hge i. simpl in *.
+    unfold Genv.find_symbol, Genv.find_def.
+    destruct ((Genv.genv_defs ge1) ! i) as [gd1 | ] eqn:Hf1; try rauto.
+    edestruct (Genv.linkorder_genv_defs Hge) as (gd2 & Hgd2 & Hgd & Hgdnp); eauto.
+    rewrite Hgd2. rauto.
+  Qed.
+
+  Global Instance find_symbol_linkorder_params:
+    Params (@Genv.find_symbol) 2.
+
+  Global Instance find_funct_ptr_linkorder:
+    Monotonic
+      (@Genv.find_funct_ptr F V)
+      (linkorder ++> - ==> option_le linkorder).
+  Proof.
+    intros ge1 ge2 Hge b. simpl in *.
+    unfold Genv.find_funct_ptr, Genv.find_def.
+    destruct Block.ident_of as [i | ]; try constructor.
+    destruct ((Genv.genv_defs ge1) ! i) as [[f1|v1] | ] eqn:Hf1; try constructor.
+    edestruct (Genv.linkorder_genv_defs Hge) as (gd2 & Hgd2 & Hgd & Hgdnp); eauto.
+    inversion Hgd; clear Hgd; subst.
+    rewrite Hgd2. rauto.
+  Qed.
+
+  Global Instance find_funct_ptr_linkorder_params:
+    Params (@Genv.find_funct_ptr) 2.
+
+  Global Instance find_var_info_linkorder:
+    Monotonic
+      (@Genv.find_var_info F V)
+      (linkorder ++> - ==> option_le linkorder).
+  Proof.
+    intros ge1 ge2 Hge b. simpl in *.
+    unfold Genv.find_var_info, Genv.find_def.
+    destruct Block.ident_of as [i | ]; try constructor.
+    destruct ((Genv.genv_defs ge1) ! i) as [[f1|v1] | ] eqn:Hf1; try constructor.
+    edestruct (Genv.linkorder_genv_defs Hge) as (gd2 & Hgd2 & Hgd & Hgdnp); eauto.
+    inversion Hgd; clear Hgd; subst.
+    rewrite Hgd2. rauto.
+  Qed.
+
+  Global Instance find_var_info_linkorder_params:
+    Params (@Genv.find_var_info) 2.
+
+  Global Instance Genv_to_senv_le:
+    Monotonic (@Genv.to_senv F V) (linkorder ++> Senv_le).
+  Proof.
+    intros ge1 ge2 Hge.
+    split; simpl; intros i.
+    - unfold Genv.find_symbol, Genv.find_def.
+      destruct ((Genv.genv_defs ge1) ! i) as [gd1 | ] eqn:Hb; [ | constructor].
+      edestruct (Genv.linkorder_genv_defs Hge) as (gd2 & Hgd2 & Hgd & _); eauto.
+      rewrite Hgd2. rauto.
+    - unfold Genv.public_symbol, Genv.find_symbol, Genv.find_def.
+      destruct ((Genv.genv_defs ge1) ! i) as [gd1 | ] eqn:Hb; [ | constructor].
+      edestruct (Genv.linkorder_genv_defs Hge) as (gd2 & Hgd2 & Hgd & _); eauto.
+      rewrite Hgd2. unfold Coqlib.proj_sumbool.
+      destruct (in_dec _ _ (_ ge1)) as [Hin | _]; try rauto.
+      eapply Genv.linkorder_genv_public in Hin; eauto.
+      destruct (in_dec _ _ (_ ge2)) as [_ | Hnotin]; try contradiction.
+      reflexivity.
+    - unfold Genv.block_is_volatile.
+      repeat rstep.
+      destruct H1. simpl. reflexivity.
+  Qed.
+
+  Global Instance genv_to_senv_params:
+    Params (@Genv.to_senv) 1.
+
+  (** * [eval_builtin_args] *)
+
+  Global Instance genv_symbol_address_linkorder:
+    Monotonic
+      (@Genv.symbol_address F V)
+      (linkorder ++> - ==> - ==> Val.lessdef).
+  Proof.
+    intros ge1 ge2 Hge id ofs.
+    unfold Genv.symbol_address.
+    repeat rstep; subst; constructor.
+  Qed.
+
+  Global Instance genv_symbol_address_linkorder_params:
+    Params (@Genv.symbol_address) 3.
+
+  Global Instance senv_symbols_address_inject:
+    Monotonic
+      (@Senv.symbol_address)
+      (Senv_le ++> - ==> - ==> Val.lessdef).
+  Proof.
+    intros ge1 ge2 Hge i ofs.
+    unfold Senv.symbol_address.
+    pose proof (Senv_le_find_symbol ge1 ge2 Hge i).
+    repeat rstep; subst; constructor.
+  Qed.
+
+  (*
+  Global Instance eval_builtin_arg_rel {F V} R w:
+    Monotonic
+      (@eval_builtin_arg)
+      (forallr -, Senv_le ++> - ==> - ==> - ==> - ==> set_le eq).
+       (- ==> eq) ++>
+       Val.inject (mi R w) ++> match_mem R w ++> - ==> set_le (Val.inject (mi R w))).
+  Proof.
+    intros A ge1 ge2 Hge f1 f2 Hf v1 v2 Hv m1 m2 Hm arg r Hr.
+    revert v2 Hv.
+    induction Hr; intros ? ?;
+    try (transport_hyps; eexists; split; [constructor; eauto | rauto]).
+    - edestruct IHHr1 as (vhi' & Hvhi' & Hvhi); eauto.
+      edestruct IHHr2 as (vlo' & Hvlo' & Hvlo); eauto.
+      eexists. split; [ constructor; eauto | rauto ].
+    - edestruct IHHr1 as (va1 & Hva1 & Hva1'); eauto.
+      edestruct IHHr2 as (va2 & Hva2 & Hva2'); eauto.
+      eexists. split; [ constructor; eauto | rauto ].
+  Qed.
+
+  Hint Extern 1 (Transport _ _ _ _ _) =>
+    set_le_transport @eval_builtin_arg : typeclass_instances.
+
+  Global Instance eval_builtin_args_rel {F V} R w:
+    Monotonic
+      (@eval_builtin_args)
+      (forallr -, (psat (genv_valid R w)) !! (@Genv.to_senv F V) ++>
+       (- ==> Val.inject (mi R w)) ++>
+       Val.inject (mi R w) ++> match_mem R w ++> - ==>
+       set_le (Val.inject_list (mi R w))).
+  Proof.
+    unfold eval_builtin_args.
+    repeat rstep.
+    intros vl Hvl.
+    induction Hvl.
+    - eexists; split; constructor; eauto.
+    - destruct IHHvl as (? & ? & ?).
+      transport H3.
+      eexists; split; constructor; eauto.
+  Qed.
+
+  Hint Extern 1 (Transport _ _ _ _ _) =>
+    set_le_transport @eval_builtin_args : typeclass_instances.
+*)
+
+
+End GENV_REL.
+
+Axiom external_call_empty :
+  forall id sg ge vargs m t vres m',
+    ~ Events.external_functions_sem id sg ge vargs m t vres m'.
+
+Axiom inline_assembly_sem_empty : (* XXX admit: or assert compatibility w/ linkorder *)
+  forall text sg ge vargs m t vres m',
+    ~ Events.inline_assembly_sem text sg ge vargs m t vres m'.
+
+Global Instance genv_block_is_volatile_linkorder:
+  Monotonic
+    (@Genv.block_is_volatile fundef unit)
+    (linkorder ++> - ==> option_le eq).
+Proof.
+  intros ge1 ge2 Hge b.
+  unfold Genv.block_is_volatile.
+  repeat rstep.
+  destruct H1. simpl. reflexivity.
+Qed.
+
+Global Instance genv_block_is_volatile_linkorder_params:
+  Params (@Genv.block_is_volatile) 2.
+
+Global Instance eventval_match_linkorder:
+  Monotonic (@Events.eventval_match) (Senv_le ++> - ==> - ==> - ==> impl).
+Proof.
+  intros ge1 ge2 Hge ev ty v H.
+  destruct H; constructor.
+  - pose proof (Senv_le_public_symbol ge1 ge2 Hge id).
+    rewrite H in H1. simpl in H1. auto.
+  - destruct (Senv_le_find_symbol ge1 ge2 Hge id); congruence.
+Qed.
+
+Global Instance eventval_list_match_linkorder:
+  Monotonic (@Events.eventval_list_match) (Senv_le ++> - ==> - ==> - ==> impl).
+Proof.
+  intros ge1 ge2 Hge ev ty v H.
+  induction H; constructor; eauto.
+  eapply eventval_match_linkorder; eauto.
+Qed.
+
+Lemma external_call_linkorder (ge1 ge2: Asm.genv) ef vargs m t vres m' :
+  linkorder ge1 ge2 ->
+  Events.external_call ef ge1 vargs m t vres m' ->
+  Events.external_call ef ge2 vargs m t vres m'.
+Proof.
+  intros Hge H.
+  destruct ef; simpl in H |- *; try now (eelim external_call_empty; eauto).
+  - destruct H; constructor.
+    destruct H.
+    + simpl in H. transport H. subst.
+      simpl in H0. transport H0. subst.
+      eapply Events.volatile_load_vol; eauto.
+      revert H1. rauto.
+    + simpl in H. transport H. subst.
+      eapply Events.volatile_load_nonvol; eauto.
+  - destruct H; constructor.
+    destruct H.
+    + simpl in H. transport H. subst.
+      simpl in H0. transport H0. subst.
+      eapply Events.volatile_store_vol; eauto.
+      revert H1. rauto.
+    + simpl in H. transport H. subst.
+      eapply Events.volatile_store_nonvol; eauto.
+  - destruct H; econstructor; eauto.
+  - destruct H; econstructor; eauto.
+  - destruct H; econstructor; eauto.
+  - destruct H; econstructor; eauto.
+    revert H. rauto.
+  - destruct H; econstructor; eauto.
+    revert H. rauto.
+  - eelim inline_assembly_sem_empty; eauto.
+  - destruct H; econstructor; eauto.
+Qed.
+
+Definition state_is_internal ge s :=
+  let '(State rs m) := s in
+  match rs#PC with
+    | Vptr b ofs => Senv.block_is_internal ge b = true
+    | _ => False
+  end.
+
+Lemma genv_fundef_is_internal (p: Asm.program):
+  Genv.genv_fundef_is_internal (Genv.globalenv p) = _.
+Proof.
+  unfold Genv.globalenv, Genv.add_globals.
+  pattern (prog_defs p).
+  eapply rev_ind.
+  - simpl. reflexivity.
+  - intros.
+    rewrite fold_left_app. simpl. auto.
+Qed.
+
+Lemma asm_step_linkorder (ge1 ge2: Asm.genv) s t s' :
+  linkorder ge1 ge2 ->
+  Genv.genv_fundef_is_internal ge1 = _ ->
+  Asm.step ge1 s t s' ->
+  Asm.step ge2 s t s'.
+Proof.
+  intros Hge Hfi Hstep.
+  destruct Hstep.
+  - transport H0.
+    inversion H4; clear H4; subst.
+    econstructor; eauto.
+  - transport H0.
+    inversion H6; clear H6; subst.
+    eapply Asm.exec_step_builtin; eauto.
+    eapply external_call_linkorder; eauto.
+  - generalize H0.
+    transport H0.
+    inversion H5; clear H5; subst.
+    + intros _.
+      eapply Asm.exec_step_external; eauto.
+      eapply external_call_linkorder; eauto.
+    + (* external -> internal *)
+      simpl in H2.
+      eelim external_call_empty; eauto.
+Qed.
 
 Section HCOMP.
   Context (p1 p2 p: Asm.program) (Hp: link p1 p2 = Some p).
@@ -45,23 +328,46 @@ Section HCOMP.
       (query_is_internal li_asm (Genv.globalenv p2) q)
       (query_is_internal li_asm (Genv.globalenv p) q).
   Proof.
+    assert (linkorder (Genv.globalenv p1) (Genv.globalenv p)) by admit.
+    assert (linkorder (Genv.globalenv p2) (Genv.globalenv p)) by admit.
+    simpl.
+    destruct q as [rs m].
+    destruct (rs PC); try constructor.
+    unfold Genv.block_is_internal.
+    unfold Genv.find_funct_ptr, Genv.find_def.
+    destruct (Block.ident_of b) as [id | ]; [ | constructor].
+    rewrite !Genv.globalenv_defs.
+    rewrite !genv_fundef_is_internal.
+    destruct (link_prog_inv p1 p2 p Hp) as (_ & Hlp & _).
+    specialize (Hlp id).
+    destruct (link_linkorder p1 p2 p Hp) as [Hp1 Hp2].
+    destruct Hp1 as (_ & _ & Hp1). specialize (Hp1 id).
+    destruct Hp2 as (_ & _ & Hp2). specialize (Hp2 id).
+    destruct ((prog_defmap p1) ! id) as [d1 | ].
+    - specialize Hp1 as (d & Hd & H1d & _); eauto.
   Admitted.
 
   Lemma internal_hcomp_l q :
     query_is_internal li_asm (Genv.globalenv p1) q = true ->
     query_is_internal li_asm (Genv.globalenv p) q = true.
-  Admitted.
+  Proof.
+    destruct (query_is_internal_cases q); congruence.
+  Qed.
 
   Lemma internal_hcomp_r q :
     query_is_internal li_asm (Genv.globalenv p2) q = true ->
     query_is_internal li_asm (Genv.globalenv p) q = true.
-  Admitted.
+  Proof.
+    destruct (query_is_internal_cases q); congruence.
+  Qed.
 
   Lemma internal_hcomp_inv q :
     query_is_internal li_asm (Genv.globalenv p) q = true ->
-    query_is_internal li_asm (Genv.globalenv p2) q = true \/
+    query_is_internal li_asm (Genv.globalenv p1) q = true \/
     query_is_internal li_asm (Genv.globalenv p2) q = true.
-  Admitted.
+  Proof.
+    destruct (query_is_internal_cases q); intuition congruence.
+  Qed.
 
   Lemma asm_hcomp_fsim_cont_l :
     fsim_match_cont cc_id (fun _ => match_states) tt
@@ -91,10 +397,6 @@ Section HCOMP.
     exists s; split; auto; repeat constructor.
   Qed.
 
-  Axiom external_call_empty :
-    forall ef ge vargs m t vres m',
-      ~ Events.external_call ef ge vargs m t vres m'.
-
   Lemma asm_hcomp_fsim :
     forward_simulation cc_id (HComp.semantics (symbolenv L) L1 L2) L.
   Proof.
@@ -115,13 +417,12 @@ Section HCOMP.
     - intros _ s12 t s12' Hs12' s Hs.
       destruct Hs12' as [s12 t s12' Hs12' | s12 r12 k12 s12' Hk12 Hs12'].
       + (* internal step *)
-        destruct Hs12' as  [si t si' kj Hsi' | si t si' kj Hsi']; simpl in *.
-      * inversion Hs; clear Hs; subst.
-        destruct Hsi'.
-        -- admit.
-        -- admit.
-        -- eelim external_call_empty; eauto.
-      * admit.
+        destruct Hs12' as  [si t si' kj Hsi' | si t si' kj Hsi']; simpl in *;
+        inversion Hs; clear Hs; subst;
+        exists si'; (split; [ | constructor]);
+        eapply asm_step_linkorder; eauto using genv_fundef_is_internal.
+        -- admit. (* linkorder *)
+        -- admit. (* linkorder *)
       + (* internal switching *)
         simpl in *.
         destruct Hk12 as [si r ki k' Hki | si r ki k' Hki]; simpl in *.
